\question \S 2.6 \# 16. Suppose that  
	\[A = \begin{bmatrix} 1 & 0 & 0 \\ 1 & 1 & 0 \\ 1 & 1 & 1\end{bmatrix}\begin{bmatrix}1 & 1 & 1 \\ 0 & 1 & 1 \\ 0 & 0 & 1\end{bmatrix}\]
	and that $b = (4,5,6)$. Solve the system $A\vec{x} = \vec{b}$ without ever calculating $A$.

	\begin{solution}
			Given $A=LU$, $A\vec{x}=\vec{b}$, and $\vec{b}=\begin{bmatrix} 4 \\ 5 \\ 6\end{bmatrix}$.  We start by solving $L\vec{c}=\vec{b}$  $\begin{bmatrix} 1 & 0 & 0 \\ 1 & 1 & 0 \\ 1 & 1 & 1\end{bmatrix}\vec{c}=\begin{bmatrix} 4 \\ 5 \\ 6\end{bmatrix}$ start by solving row one of $\vec{c}$. Since the matrix $L$ at row one, has a 1 in the first column and zeros in the rest $\vec{c}=\begin{bmatrix} 4 \\ ? \\ ?\end{bmatrix}$.  Row two of the matrix $L$ has a one in columns one and 2. So if we take 4 from the first row and subtract it from $\vec{x}$ row 2 we are left with 1. So $\vec{c}=\begin{bmatrix} 4 \\ 1 \\ ?\end{bmatrix}$  We do the same for the last row. we take rows one and two from $\vec{x}$ add them and then subtract from $\vec{b}$ which will result in $\vec{x}=\begin{bmatrix} 4 \\ 1 \\ 1\end{bmatrix}$ we now have $\vec{c}$.  We just completed forward elimination now we can use $\vec{c}$ for back substitution using the equation $U\vec{x}=\vec{c}$. We will solve this one starting with row 3 so \newline $\begin{bmatrix}1 & 1 & 1 \\ 0 & 1 & 1 \\ 0 & 0 & 1\end{bmatrix}\vec{c}=\begin{bmatrix} 4 \\ 1 \\ 1\end{bmatrix}\Rightarrow \begin{bmatrix}1 & 1 & 1 \\ 0 & 1 & 1 \\ 0 & 0 & 1\end{bmatrix}\begin{bmatrix} ? \\ ? \\ 1\end{bmatrix}=\begin{bmatrix} 4 \\ 1 \\ 1\end{bmatrix} \Rightarrow \begin{bmatrix}1 & 1 & 1 \\ 0 & 1 & 1 \\ 0 & 0 & 1\end{bmatrix}\begin{bmatrix} ? \\ 0 \\ 1\end{bmatrix}=\begin{bmatrix} 4 \\ 1 \\ 1\end{bmatrix}\Rightarrow \begin{bmatrix}1 & 1 & 1 \\ 0 & 1 & 1 \\ 0 & 0 & 1\end{bmatrix}\begin{bmatrix} 3 \\ 0 \\ 1\end{bmatrix}=\begin{bmatrix} 4 \\ 1 \\ 1\end{bmatrix}$. Therefore $A\begin{bmatrix} 3 \\ 0 \\ 1\end{bmatrix}=\begin{bmatrix} 4 \\ 5 \\ 6\end{bmatrix}.$
	\end{solution}
	