		With the projected vectors $P\vec{x}$ and $(I-P)y$ knowing $P^2=P$ and $P^T=P$. Given this we can set up the equation,
		\newline
		$(P\vec{x})^T(I-P)\vec{y}=\vec{y}$
		\newline
		$(\vec{x}^TP^T)(\vec{y}-P\vec{y})$
		\newline
		$\vec{x}^TP^T\vec{y}-\vec{x}^TP^TP\vec{y}$
		\newline
		$\vec{x}^TP\vec{y}-\vec{x}^TPP\vec{y}$
		\newline
		$\vec{x}^TP\vec{y}-\vec{x}^TP^2\vec{y}$
		\newline
		In order to be orthogonal as stated then the following equation must be true.
		\newline
		$\vec{x}^TP\vec{y}-\vec{x}^TP\vec{y}=0$
		\newline
		Projects onto the $N(A^T)$.
