				Using the projection equation and multiplying both sides by $A^T$ we can get the following.

				\begin{gather*}
				    A\hat{x}=P\vec{b}\\
				    A\hat{x}=A(A^TA)^{-1}A^T\vec{b} \\
				    A^TA\hat{x}=A^TA(A^TA)^{-1}A^T\vec{b} \\
				    A^TA\hat{x}=A^T\vec{b} \\
				\end{gather*}
				Now if we multiply by $(A^TA)^{-1}$ we can reduce the left side of the equation.
				\begin{gather*}
				    (A^TA)^{-1}A^TA\hat{x}=(A^TA)^{-1}A^T\vec{b} \\
				    \hat{x}=(A^TA)^{-1}A^T\vec{b}
				\end{gather*}

