		    Using the equation $A^TA\vec{x}=A^T\vec{b}$ we get the following. 
			    \begin{gather*}
			        \begin{bmatrix}
			        4 & -4 & -2 \\
			        1 & 5 & 1 \\
			        \end{bmatrix}
			        \begin{bmatrix}
			        4 & 1 \\
			        -4 & 5 \\
			        -2 & 1 \\
			        \end{bmatrix}
			        \vec{x}
			        =
			        \begin{bmatrix}
			        4 & -4 & -2 \\
			        1 & 5 & 1 \\
			        \end{bmatrix}
			        \begin{bmatrix}
			        1 \\
			        2 \\
			        7 \\
			        \end{bmatrix} 
			        \\
			        \begin{bmatrix}
			        36 & -18 \\
			        -18 & 27 \\
			        \end{bmatrix}
			        \vec{x}= \begin{bmatrix}
			        -18 \\
			        9 \\
			        \end{bmatrix}
			        \\
			        \begin{bmatrix}
			        36 & -18 \\
			        0 & -18 \\
			        \end{bmatrix}
			        \vec{x}= \begin{bmatrix}
			        -18 \\
			        9 \\
			        \end{bmatrix} 
			        \\
			        36x_1-18x_2=-18
			        \\
			        18x_2=9
			        \\
			        x_2=1/2
			        \\
			        x_1=-1/4
			    \end{gather*}
			    So $\vec{x}=(-1/4, 1/2)$
